Switched over to regular equality

InnerProd.v
@@ -1,4 +1,3 @@
-Require Import New.Equiv.
 Require Import New.Complex.
 Require Import New.Ring.
 Require Import New.Field.
@@ -6,8 +5,8 @@ Require Import New.Order.
 Require Import Scalars.
 Require Import States.
 
-Class InnerProdOp E S := {
-  inner_prod : E -> E -> S
+Class InnerProdOp Scalar Elem := {
+  inner_prod : Elem -> Elem -> Scalar
 }.
 
 Notation "<| x | y |>" := (inner_prod x y).
@@ -16,45 +15,50 @@ Notation "<| x | y |>" := (inner_prod x y).
  * slightly more fine-grained than those found in traditional textbooks,
  * as is necessary for mechanical proving.
  *)
-Class InnerProd E S
-  {scops : ScalarOps S}
-  {elem_sops : StateOps E S}
-  {inner_prod_ops : InnerProdOp E S} := {
-  scalars_ip :> Scalars S;
-  states_ip :> States E S;
+Class InnerProd Scalar Elem
+  {scops : ScalarOps Scalar}
+  {elem_sops : StateOps Scalar Elem}
+  {inner_prod_ops : InnerProdOp Scalar Elem} := {
+  scalars_ip :> ScalarsNoAssoc Scalar;
+  states_ip :> States Scalar Elem;
 
   (* Conjugate Symmetry of inner products *)
-  inner_prod_conj_sym : forall s1 s2 : E, <| s1 | s2 |> == ~<| s2 | s1 |>;
+  inner_prod_conj_sym : forall s1 s2 : Elem, <| s1 | s2 |> = ~<| s2 | s1 |>;
 
   (* Positivity of inner products *)
-  inner_prod_pos : forall s : E, 0 <= <| s | s |>;
+  inner_prod_pos : forall s : Elem, 0 <= <| s | s |>;
 
   (* Strictness of inner products (inner product with null is 0).
    * Left-side strictness is provable as a theorem
    *)
-  inner_prod_right_strict : forall s : E, <| s | null |> == 0;
+  inner_prod_right_strict : forall s : Elem, <| s | null |> = 0;
 
   (* Conjugate distribution of inner products *)
-  inner_prod_conj_dist : forall s1 s2 : E, <| ~s1 | ~s2 |> == ~<| s2 | s1 |>;
+  inner_prod_conj_dist : forall s1 s2 : Elem, <| ~s1 | ~s2 |> = ~<| s2 | s1 |>;
 
   (* Homogeneity of inner products *)
   inner_prod_right_homogeneous :
-    forall (s1 s2 : E) (a : S),
-      <| s1 | scalar_prod a s2 |> == a * <| s1 | s2 |>;
+    forall (s1 s2 : Elem) (a : Scalar),
+      <| s1 | scalar_prod a s2 |> = a * <| s1 | s2 |>;
 
   (* Right meet-multiply correspondance *)
   inner_prod_right_meet :
-    forall s s1 s2 : E, <| s | meet s1 s2 |> == <| s | s1 |> * <| s | s2 |>;
+    forall s s1 s2 : Elem, <| s | meet s1 s2 |> = <| s | s1 |> * <| s | s2 |>;
 
   (* Join-join property *)
   inner_prod_join :
-    forall s1 s2 s3 s4 : E,
-      <| join s1 s2 | join s3 s4 |> ==
+    forall s1 s2 s3 s4 : Elem,
+      <| join s1 s2 | join s3 s4 |> =
       <| s1 | s3 |> + <| s1 | s4 |> + <| s2 | s3 |> + <| s2 | s4 |>;
+
+  (* One-sided Join-join property *)
+  inner_prod_join_right :
+    forall s1 s2 s3 s4 : Elem,
+      <| join s1 s2 | join s3 s4 |> = <| join s1 s2 | s3 |> + <| join s1 s2 | s4 |>;
 
   (* Join-meet property *)
   inner_prod_join_meet :
-    forall s1 s2 s3 s4 : E,
-      <| join s1 s2 | meet s3 s4 |> ==
+    forall s1 s2 s3 s4 : Elem,
+      <| join s1 s2 | meet s3 s4 |> =
       (<| s1 | s3 |> + <| s2 | s3 |>) * (<| s1 | s4 |> + <| s2 | s4 |>)
 }.
