StateSpace.v
@@ -1,4 +1,3 @@
-Require Import New.Equiv.
 Require Import New.Complex.
 Require Import New.Ring.
 Require Import New.Field.
@@ -8,11 +7,23 @@ Require Import States.
 Require Import InnerProd.
 
 (* The master class containing everything *)
-Class StateSpace E S := {
-  scalarops_ss :> ScalarOps S;
-  stateops_ss :> StateOps E S;
-  innerprodop_ss :> InnerProdOp E S;
-  innerprod_ss :> InnerProd E S;
-  inner_prod_extensional_eq :
-    forall s1 s2 : E, s1 == s2 <-> (forall s : E, <| s | s1 |> == <| s | s2 |>)
+Class StateSpace Scalar State := {
+  scalarops_ss :> ScalarOps Scalar;
+  stateops_ss :> StateOps Scalar State;
+  innerprodop_ss :> InnerProdOp Scalar State;
+  innerprod_ss :> InnerProd Scalar State;
+  inner_prod_ext_ind_eq :
+    forall s1 s2 : State,
+      (forall s3 s4 : State,
+        (<| s3 | s1 |> = <| s3 | s2 |>) ->
+        (<| s4 | s1 |> = <| s4 | s2 |>) ->
+        <| join s3 s4 | s1 |> = <| join s3 s4 | s2 |>) ->
+      (forall s3 s4 : State,
+        (<| s3 | s1 |> = <| s3 | s2 |>) ->
+        (<| s4 | s1 |> = <| s4 | s2 |>) ->
+        <| meet s3 s4 | s1 |> = <| meet s3 s4 | s2 |>) ->
+      (forall s0 : State,
+        (<| s0 | s1 |> = <| s0 | s2 |>) ->
+        <| ~ s0 | s1 |> = <| ~ s0 | s2 |>) ->
+      s1 = s2
 }.
