InnerProdTheorems.v
@@ -1,6 +1,5 @@
 Module InnerProdTheorems.
 
-Require Import New.Equiv.
 Require Import New.Complex.
 Require Import New.Ring.
 Require Import Scalars.
@@ -8,154 +7,87 @@ Require Import States.
 Require Import InnerProd.
 
 (* Left homogeneity from right homogeneity and conjugate symmetry *)
-Theorem inner_prod_left_homogeneous Scalar State
+Lemma inner_prod_left_homogeneous Scalar State
   {scalarops : ScalarOps Scalar}
-  {stateops : StateOps State Scalar}
-  {innerprodop : InnerProdOp State Scalar}
-  {innerprod : InnerProd State Scalar} :
+  {stateops : StateOps Scalar State}
+  {innerprodop : InnerProdOp Scalar State}
+  {innerprod : InnerProd Scalar State} :
   forall (s1 s2 : State) (a : Scalar),
-    <| scalar_prod a s1 | s2 |> == ((~ a) * <| s1 | s2 |>).
+    <| scalar_prod a s1 | s2 |> = ((~ a) * <| s1 | s2 |>).
 Proof.
   intros.
-  apply equiv_trans with (~<| s2 | scalar_prod a s1 |>).
-  apply inner_prod_conj_sym.
-  apply equiv_trans with (~ (a * <| s2 | s1 |>)).
-  cut (<| s2 | scalar_prod a s1 |> == a * <| s2 | s1 |>).
-  apply conj_ext.
-  apply inner_prod_right_homogeneous.  
-  apply equiv_trans with ((~a) * (~<| s2 | s1 |>)).
-  generalize (<| s2 | s1 |>).
-  intro s.
-  apply equiv_trans with ((~s) * (~a)).
-  apply conj_mul.
-  apply mul_comm.
-  apply mul_extensional.
-  apply equiv_refl.
-  apply equiv_sym.
-  apply inner_prod_conj_sym.
+  rewrite inner_prod_conj_sym.
+  rewrite inner_prod_right_homogeneous.
+  rewrite conj_mul.
+  rewrite mul_comm.
+  rewrite <- inner_prod_conj_sym.
+  reflexivity.
 Qed.
 
 (* Left strictness from right strictness and conjugate symmetry *)
-Theorem inner_prod_left_strict Scalar State
+Lemma inner_prod_left_strict Scalar State
   {scalarops : ScalarOps Scalar}
-  {stateops : StateOps State Scalar}
-  {innerprodop : InnerProdOp State Scalar}
-  {innerprod : InnerProd State Scalar} :
-  forall s : State, <| null | s |> == 0.
+  {stateops : StateOps Scalar State}
+  {innerprodop : InnerProdOp Scalar State}
+  {innerprod : InnerProd Scalar State} :
+  forall s : State, <| null | s |> = 0.
 Proof.
   intro.
-  apply equiv_trans with (<| s | null |>).
-  apply equiv_trans with (~<| s | null |>).
-  apply inner_prod_conj_sym.
-  apply equiv_sym.
-  apply equiv_trans with 0.
-  apply inner_prod_right_strict.
-  apply equiv_trans with (~0).
-  apply equiv_sym.
+  rewrite inner_prod_conj_sym.
+  rewrite inner_prod_right_strict.
   apply zero_self_conj.
-  apply equiv_sym.
-  cut (<| s | null |> == 0).
-  apply conj_ext.
-  apply inner_prod_right_strict.
-  apply inner_prod_right_strict.
 Qed.
 
 (* Left meet-multiply correspondance from right meet and conjugate symmetry *)
-Theorem inner_prod_left_meet Scalar State
+Lemma inner_prod_left_meet Scalar State
   {scalarops : ScalarOps Scalar}
-  {stateops : StateOps State Scalar}
-  {innerprodop : InnerProdOp State Scalar}
-  {innerprod : InnerProd State Scalar} :
-  forall (s s1 s2 : State), <| meet s1 s2 | s |> == <| s1 | s |> * <| s2 | s |>.
+  {stateops : StateOps Scalar State}
+  {innerprodop : InnerProdOp Scalar State}
+  {innerprod : InnerProd Scalar State} :
+  forall (s s1 s2 : State), <| meet s1 s2 | s |> = <| s1 | s |> * <| s2 | s |>.
 Proof.
   intros.
-  apply equiv_trans with (~ <| s | meet s1 s2 |>).
-  apply inner_prod_conj_sym.
-  apply equiv_trans with (~(<| s | s1 |> * <| s | s2 |>)).
-  cut (<| s | meet s1 s2 |> == <| s | s1 |> * <| s | s2 |>).
-  apply conj_ext.
-  apply inner_prod_right_meet.
-  apply equiv_trans with ((~<| s | s2 |>) * (~<| s | s1 |>)).
-  apply conj_mul.
-  apply equiv_sym.
-  apply equiv_trans with ((~<| s | s1 |>) * (~<| s | s2 |>)).
-  apply mul_extensional.
-  apply inner_prod_conj_sym.
-  apply inner_prod_conj_sym.
-  apply mul_comm.
+  rewrite inner_prod_conj_sym.
+  rewrite inner_prod_right_meet.
+  rewrite conj_mul.
+  rewrite mul_comm.
+  rewrite <- 2! inner_prod_conj_sym.
+  reflexivity.
 Qed.
 
-Theorem inner_prod_meet_join Scalar State
+Lemma inner_prod_meet_join Scalar State
   {scalarops : ScalarOps Scalar}
-  {stateops : StateOps State Scalar}
-  {innerprodop : InnerProdOp State Scalar}
-  {innerprod : InnerProd State Scalar} :
+  {stateops : StateOps Scalar State}
+  {innerprodop : InnerProdOp Scalar State}
+  {innerprod : InnerProd Scalar State} :
   forall s1 s2 s3 s4 : State,
-    <| meet s1 s2 | join s3 s4 |> ==
+    <| meet s1 s2 | join s3 s4 |> =
     (<| s1 | s3 |> + <| s1 | s4 |>) * (<| s2 | s3 |> + <| s2 | s4 |>).
 Proof.
   intros.
-  apply equiv_trans with (~<| join s3 s4 | meet s1 s2 |>).
-  apply inner_prod_conj_sym.
-  apply equiv_trans with (~((<| s3 | s1 |> + <| s4 | s1 |>) *
-                           (<|s3 | s2 |> + <| s4 | s2 |>))).
-  apply conj_ext.
-  apply equiv_trans with (<| join s3 s4 | meet s1 s2 |>).
-  apply equiv_sym.
-  apply conj_inv.
-  apply equiv_trans with ((<| s3 | s1 |> + <| s4 | s1 |>) *
-                          (<| s3 | s2 |> + <| s4 | s2 |>)).
-  apply inner_prod_join_meet.
-  apply conj_inv.
-  apply equiv_trans with ((~(<| s3 | s2 |> + <| s4 | s2 |>)) *
-                          (~(<| s3 | s1 |> + <| s4 | s1 |>))).
-  apply conj_mul.
-  apply equiv_trans with ((~ <| s3 | s1 |> + <| s4 | s1 |>) *
-                          (~ <| s3 | s2 |> + <| s4 | s2 |>)).
-  apply mul_comm.
-  apply equiv_trans with (((~ <| s3 | s1 |>) + (~ <| s4 | s1 |>)) *
-                          (~(<| s3 | s2 |> + <| s4 | s2 |>))).
-  apply mul_extensional.
-  apply conj_sum.
-  apply equiv_refl.
-  apply equiv_trans with (((~ <| s3 | s1 |>) + (~ <| s4 | s1 |>)) *
-                          ((~ <| s3 | s2 |>) + (~ <| s4 | s2 |>))).
-  apply mul_extensional.
-  apply equiv_refl.
-  apply conj_sum.
-  apply equiv_trans with ((<| s1 | s3 |> + (~ <| s4 | s1 |>)) *
-                          ((~ <| s3 | s2 |>) + (~ <| s4 | s2 |>))).
-  apply mul_extensional.
-  apply add_extensional.
-  apply equiv_sym.
-  apply inner_prod_conj_sym.
-  apply equiv_refl.
-  apply equiv_refl.
-  apply equiv_trans with ((<| s1 | s3 |> + <| s1 | s4 |>) *
-                          ((~ <| s3 | s2 |>) + (~ <| s4 | s2 |>))).
-  apply mul_extensional.
-  apply add_extensional.
-  apply equiv_refl.
-  apply equiv_sym.
-  apply inner_prod_conj_sym.
-  apply equiv_refl.
-  apply equiv_trans with ((<| s1 | s3 |> + <| s1 | s4 |>) *
-                          (<| s2 | s3 |> + (~ <| s4 | s2 |>))).
-  apply mul_extensional.
-  apply equiv_refl.
-  apply add_extensional.
-  apply equiv_sym.
-  apply inner_prod_conj_sym.
-  apply equiv_refl.
-  apply equiv_trans with ((<| s1 | s3 |> + <| s1 | s4 |>) *
-                          (<| s2 | s3 |> + <| s2 | s4 |>)).
-  apply mul_extensional.
-  apply equiv_refl.
-  apply add_extensional.
-  apply equiv_refl.
-  apply equiv_sym.
-  apply inner_prod_conj_sym.
-  apply equiv_refl.
+  rewrite inner_prod_conj_sym.
+  rewrite inner_prod_join_meet.
+  rewrite conj_mul.
+  rewrite mul_comm.
+  rewrite 2! conj_sum.
+  rewrite <- 4! inner_prod_conj_sym.
+  reflexivity.
+Qed.
+
+Lemma inner_prod_join_left Scalar State
+  {scalarops : ScalarOps Scalar}
+  {stateops : StateOps Scalar State}
+  {innerprodop : InnerProdOp Scalar State}
+  {innerprod : InnerProd Scalar State} :
+    forall s1 s2 s3 s4 : State,
+      <| join s1 s2 | join s3 s4 |> = <| s1 | join s3 s4 |> + <| s2 | join s3 s4 |>.
+Proof.
+  intros.
+  rewrite inner_prod_conj_sym.
+  rewrite inner_prod_join_right.
+  rewrite conj_sum.
+  rewrite <- 2! inner_prod_conj_sym.
+  reflexivity.
 Qed.
 
 End InnerProdTheorems.
