StateSpaceTheorems.v
@@ -1,0 +1,31 @@
+Module StateSpaceTheorems.
+
+Require Import Setoid.
+Require Import New.Complex.
+Require Import New.Equiv.
+Require Import New.Ring.
+Require Import New.RingTheorems.
+Require Import New.Field.
+Require Import InnerProd.
+Require Import Scalars.
+Require Import States.
+Require Import StateSpace.
+
+
+Lemma state_join_bot Scalar State
+  {statespace : StateSpace Scalar State} :
+  forall (s : State), join null s = s.
+Proof.
+  intros.
+  apply inner_prod_ext_ind_eq.
+  intros.
+  rewrite inner_prod_join.
+  rewrite 2! inner_prod_right_strict.
+  rewrite add_zero_right.
+  rewrite add_zero_left.
+  rewrite <- inner_prod_join.
+  rewrite add_comm at 1.
+  intro.
+Qed.
+
+End StateSpaceTheorems.
